Replace `BlockPtr.link{Next,Prev}Block` with `linkBetween`

Veir/Rewriter/LinkedList/Basic.lean
@@ -151,65 +151,34 @@ theorem OperationPtr.linkBetweenWithParent_fieldsInBounds (hx : ctx.FieldsInBoun
   Block linked list.
 -/
 
-/--
-  Add previous and next links to `newBlock`, linking it after `self`.
-  In particular, this does not update any parent pointers.
--/
 @[irreducible]
-def BlockPtr.linkNextBlock (self: BlockPtr) (ctx: IRContext) (newBlock: BlockPtr)
-    (opIn: self.InBounds ctx := by grind)
-    (newBlockIn: newBlock.InBounds ctx := by grind)
-    (ctxInBounds: ctx.FieldsInBounds := by grind) : IRContext :=
-  let nextBlock := (self.get ctx).next
-  -- Set the new op's next and previous pointers
-  let ctx := newBlock.setPrevBlock ctx (some self)
-  let ctx := newBlock.setNextBlock ctx nextBlock
-  -- Update self
-  let ctx := self.setNextBlock ctx (some newBlock)
-  -- Update next op if it exists
-  match heq : nextBlock with
-  | none => ctx
-  | some nextOp => nextOp.setPrevBlock ctx (some newBlock) (by grind (ematch := 10))
+def BlockPtr.linkBetween (self: BlockPtr) (ctx: IRContext)
+    (prevBlock: Option BlockPtr) (nextBlock: Option BlockPtr)
+    (selfIn: self.InBounds ctx := by grind)
+    (prevIn: ∀ prev, prevBlock = some prev → (prev.InBounds ctx) := by grind)
+    (nextIn: ∀ next, nextBlock = some next → (next.InBounds ctx) := by grind) : IRContext :=
+  let ctx := self.setPrevBlock ctx prevBlock
+  let ctx := self.setNextBlock ctx nextBlock
+    match _ : prevBlock with
+    | none =>
+      match _ : nextBlock with
+      | none => ctx
+      | some nextOp => nextOp.setPrevBlock ctx (some self)
+    | some prevOp =>
+      let ctx := prevOp.setNextBlock ctx (some self)
+      match _ : nextBlock with
+      | none => ctx
+      | some nextOp => nextOp.setPrevBlock ctx (some self)
 
 @[grind =]
-theorem BlockPtr.linkNextBlock_inBounds (ptr : GenericPtr) :
-    ptr.InBounds (linkNextBlock self ctx newBlock h₁ h₂ h₃) ↔ ptr.InBounds ctx := by
-  simp [linkNextBlock] <;> grind
+theorem BlockPtr.linkBetween_inBounds (ptr : GenericPtr) :
+    ptr.InBounds (linkBetween self ctx prevBlock nextBlock h₁ h₂ h₃) ↔ ptr.InBounds ctx := by
+  unfold linkBetween; grind
 
 @[grind .]
-theorem BlockPtr.linkNextBlock_fieldsInBounds :
-    (linkNextBlock self ctx newBlock h₁ h₂ h₃).FieldsInBounds := by
-  grind [linkNextBlock]
-
-/--
-  Add previous and next links to `newOp`, linking it before `self`.
-  In particular, this does not update any parent pointers.
--/
-@[irreducible]
-def BlockPtr.linkPrevBlock (self: BlockPtr) (ctx: IRContext) (newBlock: BlockPtr)
-    (opIn: self.InBounds ctx := by grind)
-    (newBlockIn: newBlock.InBounds ctx := by grind)
-    (ctxInBounds: ctx.FieldsInBounds := by grind) : IRContext :=
-  let prevOp := (self.get ctx).prev
-  -- Set the new op's next and previous pointers
-  let ctx := newBlock.setNextBlock ctx (some self)
-  let ctx := newBlock.setPrevBlock ctx prevOp
-  -- Update self
-  let ctx := self.setPrevBlock ctx (some newBlock)
-  -- Update previous op if it exists
-  match heq : prevOp with
-  | none => ctx
-  | some prevOp => prevOp.setNextBlock ctx (some newBlock) (by grind (ematch := 10))
-@[grind =]
-theorem BlockPtr.linkPrevBlock_inBounds (ptr : GenericPtr) :
-    ptr.InBounds (linkPrevBlock self ctx newBlock h₁ h₂ h₃) ↔ ptr.InBounds ctx := by
-  simp [linkPrevBlock] <;> grind
-
-@[grind .]
-theorem BlockPtr.linkPrevBlock_fieldsInBounds :
-    (linkPrevBlock self ctx newBlock h₁ h₂ h₃).FieldsInBounds := by
-  grind [linkPrevBlock]
-
+theorem BlockPtr.linkBetween_fieldsInBounds (hx : ctx.FieldsInBounds) :
+    (linkBetween self ctx prevBlock nextBlock h₁ h₂ h₃).FieldsInBounds := by
+  unfold linkBetween; simp only; split <;> grind
 /--
   Set `self` parent to be `parent`.
   Checks that `self` does not already have a parent.
@@ -223,13 +192,56 @@ def BlockPtr.setParentWithCheck (self: BlockPtr) (ctx: IRContext) (parent: Regio
   | none => self.setParent ctx (some parent)
 
 @[grind .]
-theorem BlockPtr.setParentWithCheck_inBounds (ptr :
-    GenericPtr) (h : ptr.InBounds ctx) (heq : setParentWithCheck self ctx parent h₁ = some ctx') :
-    ptr.InBounds ctx' := by
-  simp [setParentWithCheck] at * <;> grind
-
-@[grind .]
 theorem BlockPtr.setParentWithCheck_fieldsInBounds
     (h₁ : ctx.FieldsInBounds) (h₂ : self.InBounds ctx) (h₃ : parent.InBounds ctx) :
     (setParentWithCheck self ctx parent h₂).maybe₁ IRContext.FieldsInBounds := by
   grind [setParentWithCheck, Option.maybe₁]
+
+@[grind =>]
+theorem BlockPtr.setParentWithCheck_fieldsInBounds_some
+    (h₁ : ctx.FieldsInBounds) (h₂ : self.InBounds ctx) (h₃ : parent.InBounds ctx)
+    (heq : setParentWithCheck self ctx parent h₂ = some newCtx) :
+    newCtx.FieldsInBounds := by
+  grind [setParentWithCheck, Option.maybe₁]
+
+@[grind =>]
+theorem BlockPtr.setParentWithCheck_inBounds (ptr : GenericPtr)
+    (h : self.InBounds ctx)
+    (heq : setParentWithCheck self ctx parent h = some newCtx) :
+    ptr.InBounds newCtx ↔ ptr.InBounds ctx := by
+  grind [setParentWithCheck]
+
+@[irreducible]
+def BlockPtr.linkBetweenWithParent (self: BlockPtr) (ctx: IRContext)
+    (prevBlock: Option BlockPtr) (nextBlock: Option BlockPtr)
+    (parent: RegionPtr)
+    (selfIn: self.InBounds ctx := by grind)
+    (prevIn: ∀ prev, prevBlock = some prev → (prev.InBounds ctx) := by grind)
+    (nextIn: ∀ next, nextBlock = some next → (next.InBounds ctx) := by grind)
+    (parentIn : parent.InBounds ctx := by grind) : Option IRContext :=
+  let ctx := self.linkBetween ctx prevBlock nextBlock
+  rlet ctx ← self.setParentWithCheck ctx parent
+  match _ : prevBlock with
+    | none =>
+      let ctx := parent.setFirstBlock ctx (some self)
+      match _ : nextBlock with
+      | none => parent.setLastBlock ctx (some self)
+      | some nextBlock => ctx
+    | some prevBlock =>
+      match _ : nextBlock with
+      | none => parent.setLastBlock ctx (some self)
+      | some nextBlock => ctx
+
+@[grind .]
+theorem BlockPtr.linkBetweenWithParent_inBounds (ptr : GenericPtr)
+    (heq : linkBetweenWithParent self ctx prevBlock nextBlock parent h₁ h₂ h₃ h₄ = some newCtx) :
+    ptr.InBounds newCtx ↔ ptr.InBounds ctx := by
+  unfold linkBetweenWithParent at heq
+  grind
+
+@[grind .]
+theorem BlockPtr.linkBetweenWithParent_fieldsInBounds (hx : ctx.FieldsInBounds)
+    (heq : linkBetweenWithParent self ctx prevBlock nextBlock parent h₁ h₂ h₃ h₄ = some newCtx) :
+    newCtx.FieldsInBounds := by
+  unfold linkBetweenWithParent at heq
+  split at heq <;> grind
